Java/src/Logic/ST.v
@@ -37,70 +37,91 @@ Fixpoint subst_ST (x : var) (v : val) (t : ST) : ST :=
 
 Definition subst_STs (x : var) (v : val) (t : STs) : STs := map (subst_ST x v) t.
 
-Inductive ST_trace : Prog_wf -> traces -> ST -> trace -> Prop :=
-  | stt_init : forall (p : Prog_wf) (trs : traces), ST_trace p trs st_end tinit
-  | stt_send : forall (p : Prog_wf) (trs : traces) (t : ST) (v : val) (h : heap) (tr : trace)
+Inductive ST_trace : Prog_wf -> ST -> trace -> Prop :=
+  | stt_init : forall (p : Prog_wf), ST_trace p st_end tinit
+  | stt_send : forall (p : Prog_wf) (t : ST) (v : val) (h : heap) (tr : trace)
   			   (HGuard: forall (x : var) (A : sasn) (t' : ST),
   			     t = (st_send x A t') ->
-  			     (apply_subst A (subst1 `v  x)) (stack_empty var) trs p O h -> 
-  			     ST_trace p trs (subst_ST x v t') tr
+  			     (apply_subst A (subst1 `v  x)) (stack_empty var) (empty _) p O h -> 
+  			     ST_trace p (subst_ST x v t') tr
   			   ),
-               ST_trace p trs t (tsend v h tr)
-  | stt_recv : forall (p : Prog_wf) (trs : traces) (t : ST) (v : val) (h : heap) (tr : trace)
+               ST_trace p t (tsend v h tr)
+  | stt_recv : forall (p : Prog_wf) (t : ST) (v : val) (h : heap) (tr : trace)
   			   (HGuard: forall (x : var) (A : sasn) (t' : ST),
   			     t = (st_recv x A t') ->
-  			     (apply_subst A (subst1 `v  x)) (stack_empty var) trs p O h /\ 
-  			     ST_trace p trs (subst_ST x v t') tr
+  			     (apply_subst A (subst1 `v  x)) (stack_empty var) (empty _) p O h /\ 
+  			     ST_trace p (subst_ST x v t') tr
   			   ),
-               ST_trace p trs t (trecv v h tr)
+               ST_trace p t (trecv v h tr)
   .
+
+Inductive ST_trace_strong : Prog_wf -> ST -> trace -> Prop :=
+  | stt_init_strong : forall (p : Prog_wf), ST_trace_strong p st_end tinit
+  | stt_send_strong : forall (p : Prog_wf) (t : ST) (v : val) (h : heap) (x : var) (A : sasn) (tr : trace)
+                      (HAsn : (apply_subst A (subst1 `v  x)) (stack_empty var) (empty _) p O h),
+                      ST_trace_strong p (subst_ST x v t) tr ->
+                      ST_trace_strong p (st_send x A t) (tsend v h tr)
+  | stt_recv_strong : forall (p : Prog_wf) (t : ST) (v : val) (h : heap) (x : var) (A : sasn) (tr : trace)
+                      (HAsn : (apply_subst A (subst1 `v  x)) (stack_empty var) (empty _) p O h),
+                      ST_trace_strong p (subst_ST x v t) tr ->
+                      ST_trace_strong p (st_recv x A t) (trecv v h tr)
+  .
+
+Lemma subst_ST_dual_comm : forall (t : ST) (x : var) (v : val),
+	dual (subst_ST x v t) = subst_ST x v (dual t).
+Proof.
+  intros; unfold dual in *.
+  induction t; simpl; [reflexivity |..];
+  rewrite IHt; reflexivity.
+Qed.
+
+Lemma ST_trace_strong_dual : forall (p : Prog_wf) (t : ST) (tr : trace),
+							 ST_trace_strong p t tr ->
+							 ST_trace_strong p (dual t) (dual tr).
+Proof.
+  intros.
+  induction H; constructor; try assumption;
+  unfold dual in *; simpl;
+  rewrite <- subst_ST_dual_comm;
+  apply IHST_trace_strong.
+Qed.
+
+Lemma ST_trace_strong_weakening : forall (p : Prog_wf) (t : ST) (tr : trace),
+							      ST_trace_strong p t tr ->
+							      ST_trace        p t tr.
+Proof.
+  intros.
+  induction H; constructor; intros;
+  inversion H0; subst; [| split]; assumption.
+Qed.
 
 Local Transparent ILPre_Ops.
 Local Transparent ILFun_Ops.
 Local Transparent BILPre_Ops.
 Local Transparent BILFun_Ops.
 
-Instance ST_trace_m : Proper (eq ==> Equal ==> eq ==> eq ==> iff) ST_trace.
+Instance ST_trace_strong_subprog_m : Proper (Prog_wf_sub ==> eq ==> eq ==> impl) ST_trace_strong.
 Proof.
-  intros P P' HPP' trs trs' HtrsEqual tr tr' Htreq t t' Hteq.
-  split; intro Hstt; subst.
-  - induction Hstt.
-    * apply stt_init.
-    * apply stt_send.
-      intros.
-      apply H with (A := A); [ apply H0 | | apply HtrsEqual ].
-      solve_model H1; [| congruence].
-      symmetry; apply HtrsEqual.
-    * apply stt_recv.
-      intros.
-      specialize (HGuard _ _ _ H).
-      destruct HGuard as [HP Hstt].
-      split.
-      + solve_model HP; congruence.
-      + admit (* fangel *).
-  - induction Hstt.
-    * apply stt_init.
-    * apply stt_send.
-      intros.
-      apply H with (A := A); [ apply H0 | | apply HtrsEqual ].
-      solve_model H1; congruence.
-    * apply stt_recv.
-      intros.
-      specialize (HGuard _ _ _ H).
-      destruct HGuard as [HP Hstt].
-      split.
-      + solve_model HP; congruence.
-      + admit (* fangel *).
+  intros P P' HPP st st' Htreq tr tr' Hteq H; subst.
+  generalize dependent st'.
+  induction tr'; intros st' H; inversion H; subst.
+  - constructor.
+  - constructor.
+    solve_model HAsn; congruence.
+    apply IHtr'; assumption.
+  - constructor.
+    solve_model HAsn; congruence.
+    apply IHtr'; assumption.
 Qed.
 
 Definition STs_traces (P : Prog_wf) (t : STs) (tr : traces) : Prop := forall k t', 
-  MapsTo k t' t -> exists tr', MapsTo k tr' tr /\ ST_trace P (remove k tr) t' tr'.
+  MapsTo k t' t -> exists tr', MapsTo k tr' tr /\ ST_trace P t' tr'.
 
-Program Definition has_ST (c : val) (t : ST) : tasn := 
-  mk_tasn (fun trs => mk_asn (fun P k h => forall P' tr, 
+Program Definition has_ST (c : expr) (t : open ST) : sasn := 
+  fun s => mk_tasn (fun trs => mk_asn (fun P k h => forall P' tr, 
     Prog_wf_sub P P' -> 
-    MapsTo (val_to_stptr c) tr trs -> 
-    ST_trace P' (remove (val_to_stptr c) trs) t tr
+    MapsTo (val_to_stptr (c s)) tr trs -> 
+    ST_trace P' (t s) tr
   ) _ _ _) _.
 Next Obligation.
   assert (Prog_wf_sub P P'0).
@@ -109,14 +130,12 @@ Next Obligation.
 Defined.
 Next Obligation.
   rewrite <- H in H2.
-  rewrite <- H.
   apply H0; assumption.
 Defined.
 
 Module STNotations.
-  
-	Notation " x ':' t " := (has_ST x t) (at level 88, left associativity) : st_scope.
-
+  	Notation " x ':' t " := (has_ST x t) (at level 88, left associativity) : st_scope.
+  	
 	Notation " '!' x ',{' P '}.' t " := (st_send x P t) (at level 88, left associativity) : st_scope.
 	Notation " '&' x ',{' P '}.' t " := (st_recv x P t) (at level 88, left associativity) : st_scope.
 
