Java/src/Semantics/OperationalSemantics.v
@@ -1,7 +1,7 @@
-Require Import Program SepAlg SepAlgInsts Heap AssertionLogic SpecLogic SepAlgMap.
+Require Import Program SepAlg SepAlgInsts Heap ProtocolLogic AssertionLogic SpecLogic SepAlgMap.
 Require Import MapInterface MapFacts.
-Require Import ILInsts ILogic ILEmbed ILEmbedTac ILQuantTac OpenILogic 
-        Open Subst Stack Lang SemCmd HeapArr Traces ST SemCmdRules BILogic.
+Require Import ILInsts ILogic ILEmbed ILEmbedTac ILQuantTac OpenILogic
+               Open Subst Stack Lang SemCmd HeapArr Traces ST SemCmdRules BILogic.
 
 Import SepAlgNotations.
 
@@ -11,9 +11,9 @@ Unset Strict Implicit.
 Section Commands.
 
   Inductive assign_sem (x : var) (e : dexpr) : semCmdType :=
-  | assign_ok : forall P s h t v
+  | assign_ok : forall P PM s h t v
                        (He: eval e s = v),
-      assign_sem x e P 1 s h t (Some (stack_add x v s, (h, t))).
+      assign_sem x e P PM 1 s h t (Some (stack_add x v s, (h, t))).
   Program Definition assign_cmd x e := Build_semCmd (assign_sem x e) _ _.
   Next Obligation.
     intros H; inversion H.
@@ -24,14 +24,14 @@ Section Commands.
   Qed.
 
   Inductive read_sem (x y : var) (f : field) : semCmdType :=
-  | read_ok : forall ref v P (s : stack) (h : heap) (t : traces)
+  | read_ok : forall ref v P PM (s : stack) (h : heap) (t : traces)
       (Rref  : s y = vptr ref)
       (Rmaps : MapsTo (ref,f) v (get_heap_ptr h)),
-      read_sem x y f P 1 s h t (Some (stack_add x v s, (h, t)))
-  | read_fail : forall ref P s (h : heap) (t : traces)
+      read_sem x y f P PM 1 s h t (Some (stack_add x v s, (h, t)))
+  | read_fail : forall ref P PM s (h : heap) (t : traces)
       (Sref   : s y = vptr ref)
       (Snotin : ~ In (ref,f) (get_heap_ptr h)),
-      read_sem x y f P 1 s h t None.
+      read_sem x y f P PM 1 s h t None.
   Program Definition read_cmd x y f := Build_semCmd (read_sem x y f) _ _.
   Next Obligation.
     intros H; inversion H.
@@ -119,17 +119,17 @@ Require Import Compare_dec.
     List.Forall (fun v => exists a, v = vint a /\ (a >= 0)%Z) vpath.
 *)
   Inductive read_arr_sem (x y : var) (path : list dexpr) : semCmdType :=
-  | read_arr_ok P arr s h t v vpath
+  | read_arr_ok P PM arr s h t v vpath
                 (Sref : s y = varr arr)
                 (Smap : List.map (fun e => eval e s) path = vpath)
 (*                (Sarr : valid_path vpath)*)
                 (Sfind : find_heap_arr arr (List.map val_to_nat vpath) (get_heap_arr h) = Some v) :
-      read_arr_sem x y path P 1 s h t (Some (stack_add x v s, (h, t)))
-  | read_arr_fail P arr s h t vpath
+      read_arr_sem x y path P PM 1 s h t (Some (stack_add x v s, (h, t)))
+  | read_arr_fail P PM arr s h t vpath
                   (Sref : s y = varr arr)
                   (Smap : List.map (fun e => eval e s) path = vpath)
                   (Sarr : ~ in_heap_arr arr (List.map val_to_nat vpath) (get_heap_arr h)) :
-      read_arr_sem x y path P 1 s h t None.
+      read_arr_sem x y path P PM 1 s h t None.
   Program Definition read_arr_cmd x y path := Build_semCmd (read_arr_sem x y path) _ _.
   Next Obligation.
     intros H. inversion H.
@@ -148,17 +148,17 @@ Require Import Compare_dec.
   Qed.
 
   Inductive write_arr_sem (x : var) (path : list dexpr) (e : dexpr) : semCmdType :=
-  | write_arr_ok P arr s h ha' t vpath
+  | write_arr_ok P PM arr s h ha' t vpath
                  (Sref : s x = varr arr)
                  (Smap : List.map (fun e' => eval e' s) path = vpath)
                  (Sin  : in_heap_arr arr (List.map val_to_nat vpath) (get_heap_arr h))
                  (Sha  : add_heap_arr arr (List.map val_to_nat vpath) (get_heap_arr h) (eval e s) = Some ha') :
-      write_arr_sem x path e P 1 s h t (Some (s, ((mkheap (get_heap_ptr h) ha'), t)))
-  | write_arr_fail P arr s h t vpath
+      write_arr_sem x path e P PM 1 s h t (Some (s, ((mkheap (get_heap_ptr h) ha'), t)))
+  | write_arr_fail P PM arr s h t vpath
                    (Sref : s x = varr arr)
                    (Smap : List.map (fun e' => eval e' s) path = vpath)
                    (Sin  : ~ in_heap_arr arr (List.map val_to_nat vpath) (get_heap_arr h)) :
-      write_arr_sem x path e P 1 s h t None.
+      write_arr_sem x path e P PM 1 s h t None.
   Program Definition write_arr_cmd x path e := Build_semCmd (write_arr_sem x path e) _ _.
   Next Obligation.
     intros H. inversion H.
@@ -183,11 +183,11 @@ Require Import Compare_dec.
   Qed.
 
   Inductive alloc_arr_sem (x : var) (e : dexpr) : semCmdType :=
-  | alloc_arr_ok (P : Prog_wf) (s s' : stack) (h : heap) (ha' : heap_arr) (t : traces) (n : nat)
+  | alloc_arr_ok (P : Prog_wf) PM (s s' : stack) (h : heap) (ha' : heap_arr) (t : traces) (n : nat)
                  (Sfresh_ha : forall i, ~ In (n, i) (get_heap_arr h)) 
                  (Sha : alloc_heap_arr n (val_to_nat (eval e s)) (get_heap_arr h) === ha') 
                  (Ss : s' = stack_add x (varr n) s) :
-      alloc_arr_sem x e P 1 s h t (Some (s', ((mkheap (get_heap_ptr h) ha'), t))).
+      alloc_arr_sem x e P PM 1 s h t (Some (s', ((mkheap (get_heap_ptr h) ha'), t))).
   Program Definition alloc_arr_cmd x e := Build_semCmd (alloc_arr_sem x e) _ _.
   Next Obligation.
     intros H; inversion H.
@@ -231,14 +231,14 @@ Require Import Compare_dec.
   Qed.
     
   Inductive alloc_sem (x : var) (C : class) : semCmdType :=
-  | alloc_ok : forall (P : Prog_wf) (s s' : stack) (h : heap) (hp' : heap_ptr) t n fields
+  | alloc_ok : forall (P : Prog_wf) PM (s s' : stack) (h : heap) (hp' : heap_ptr) t n fields
       (Snotnull : (n, C) <> pnull)
       (Sfresh_h : forall f, ~ In ((n, C), f) (get_heap_ptr h))
       (Sfields  : field_lookup P C fields)
       (Sh0      : sa_mul (get_heap_ptr h)
         (SS.fold (fun f h' => add ((n, C), f) (pnull : val) h') fields heap_ptr_unit) hp')
       (Ss0      : s' = stack_add x (vptr (n, C)) s),
-      alloc_sem x C P 1 s h t (Some (s', ((mkheap hp' (get_heap_arr h)), t))).
+      alloc_sem x C P PM 1 s h t (Some (s', ((mkheap hp' (get_heap_arr h)), t))).
   Program Definition alloc_cmd x C := Build_semCmd (alloc_sem x C) _ _.
   Next Obligation.
     intros H; inversion H.
@@ -263,16 +263,16 @@ Require Import Compare_dec.
   Qed.
 
   Inductive write_sem (x:var) (f:field) (e:dexpr) : semCmdType := 
-  | write_ok : forall P (s: stack) (h : heap) (hp' : heap_ptr) t ref v
+  | write_ok : forall P PM (s: stack) (h : heap) (hp' : heap_ptr) t ref v
       (Sref: s x = vptr ref)
       (Sin:  In (ref,f) (get_heap_ptr h) )
       (Heval : eval e s = v)
       (Sadd: hp' = add (ref,f) v (get_heap_ptr h) ),
-      write_sem x f e P 1 s h t (Some (s, ((mkheap hp' (get_heap_arr h)), t)))
-  | write_fail : forall P (s: stack) h t ref
+      write_sem x f e P PM 1 s h t (Some (s, ((mkheap hp' (get_heap_arr h)), t)))
+  | write_fail : forall P PM (s: stack) h t ref
       (Sref:   s x = vptr ref)
       (Sin : ~ In (ref, f) (get_heap_ptr h)),
-      write_sem x f e P 1 s h t None.
+      write_sem x f e P PM 1 s h t None.
   Program Definition write_cmd x f e := Build_semCmd (write_sem x f e) _ _.
   Next Obligation.
     intros H; inversion H.
@@ -295,18 +295,18 @@ Require Import Compare_dec.
   Qed.
 
   Inductive send_sem (x v : var) : semCmdType :=
-  | send_ok : forall P (s: stack) (h mres: heap) (t t': traces) (tr: trace) (c: stptr)
+  | send_ok : forall P PM (s: stack) (h mres: heap) (t t': traces) (tr: trace) (c: stptr)
     (Sref: s x = vst c)
     (Strace: MapsTo c (tsend (s v) mres tr) t)
     (Smarshall: marshall (s v) h mres)
     (Sadd: t' = add c tr t),
-    send_sem x v P 1 s h t (Some (s, (h, t')))
-  | send_fail2 : forall P (s: stack) (h mres: heap) (t: traces) (tr: trace) (c: stptr)
+    send_sem x v P PM 1 s h t (Some (s, (h, t')))
+  | send_fail2 : forall P PM (s: stack) (h mres: heap) (t: traces) (tr: trace) (c: stptr)
   	(Sref: s x = vst c)
     (Strace: MapsTo c (tsend (s v) mres tr) t)
     (Smarshalls: ~ marshall (s v) h mres),
     (* Unable to marshall the value pointed to by (s v) in the heap h *)
-    send_sem x v P 1 s h t None
+    send_sem x v P PM 1 s h t None
   .  
   Program Definition send_cmd x v := Build_semCmd (send_sem x v) _ _.
   Next Obligation.
@@ -331,12 +331,12 @@ Require Import Compare_dec.
   Qed.
 
   Inductive recv_sem (v x : var) : semCmdType :=
-  | recv_ok : forall P (s: stack) (h rh h': heap) (t t': traces) (tr: trace) (c: stptr) (rv : sval)
+  | recv_ok : forall P PM (s: stack) (h rh h': heap) (t t': traces) (tr: trace) (c: stptr) (rv : sval)
     (Sref: s x = vst c)
     (Strace: MapsTo c (trecv rv rh tr) t)
     (Snewheap : sa_mul h rh h')
     (Sadd: t' = add c tr t),
-    recv_sem v x P 1 s h t (Some (stack_add v rv s, (h', t')))
+    recv_sem v x P PM 1 s h t (Some (stack_add v rv s, (h', t')))
   .
   Program Definition recv_cmd v x := Build_semCmd (recv_sem v x) _ _.
   Next Obligation.
@@ -380,23 +380,23 @@ Require Import Compare_dec.
         
   Inductive call_sem (rvar : var) (C : open class) m es (c : cmd) (sc : semCmd)
     : semCmdType :=
-  | call_failS : forall (P : Prog_wf) s h t
+  | call_failS : forall (P : Prog_wf) PM s h t
       (HLFail  : forall mrec, ~ method_lookup P (C s) m mrec),
-      call_sem rvar C m es c sc P 1 s h t None
-  | call_failC : forall (P : Prog_wf) ps rexpr (s : stack) h t n
+      call_sem rvar C m es c sc P PM 1 s h t None
+  | call_failC : forall (P : Prog_wf) PM ps rexpr (s : stack) h t n
       (HLookup : method_lookup P (C s) m (Build_Method ps c rexpr))
       (HLen    : length ps = length es)
-      (HFail   : sc P n (create_stack ps (eval_exprs s es)) h t None),
-      call_sem rvar C m es c sc P (S n) s h t None
-  | call_failL : forall (P : Prog_wf) ps rexpr s h t
+      (HFail   : sc P PM n (create_stack ps (eval_exprs s es)) h t None),
+      call_sem rvar C m es c sc P PM (S n) s h t None
+  | call_failL : forall (P : Prog_wf) PM ps rexpr s h t
       (HLookup : method_lookup P (C s) m (Build_Method ps c rexpr))
       (HLen    : length ps <> length es),
-      call_sem rvar C m es c sc P 1 s h t None
-  | call_ok    : forall (P : Prog_wf) ps rexpr (s sr : stack) (h hr : heap) (t tr : traces) n
+      call_sem rvar C m es c sc P PM 1 s h t None
+  | call_ok    : forall (P : Prog_wf) PM ps rexpr (s sr : stack) (h hr : heap) (t tr : traces) n
       (HLookup : method_lookup P (C s) m (Build_Method ps c rexpr))
       (HLen    : length ps = length es)
-      (HSem    : sc P n (create_stack ps (eval_exprs s es)) h t (Some (sr, (hr, tr)))),
-      call_sem rvar C m es c sc P (S n) s h t
+      (HSem    : sc P PM n (create_stack ps (eval_exprs s es)) h t (Some (sr, (hr, tr)))),
+      call_sem rvar C m es c sc P PM (S n) s h t
         (Some (stack_add rvar (eval rexpr sr) s, (hr, tr))).
   Program Definition call_cmd rvar C m es c sc := Build_semCmd (call_sem rvar C m es c sc) _ _.
   Next Obligation.
@@ -409,14 +409,28 @@ Require Import Compare_dec.
     intros k HLe HFail; apply HSafe with (S k); [omega |]...
   Qed.
   
-  Inductive start_sem (C : class) (m : method) (x : var) (c : cmd) (sc : semCmd)
+  Inductive start_sem (C : class) (m : method) (x : var) (p : protocol) (c : cmd) (sc : semCmd)
     : semCmdType :=
-  | start_ok    : forall (P : Prog_wf) (a : var) (chan : stptr) (s rs: stack) (h rh : heap) (trs rtrs : traces) (tr : trace) (rexpr : dexpr) n
-       (HFresh  : ~ In chan trs)
-       (HLookup : method_lookup P C m (Build_Method (a::nil) c rexpr))
-       (HSem    : sc P n (stack_add a (vst chan) (stack_empty _)) heap_unit (add chan tr (empty _)) (Some (rs, (rh, rtrs)))),
-       start_sem C m x c sc P (S n) s h trs (Some ((stack_add x (vst chan) s), (h, (add chan (dual tr) trs)))).
-  Program Definition start_cmd C m x c sc := Build_semCmd (start_sem C m x c sc) _ _.
+  | start_failM   : forall (P : Prog_wf) PM (a : var) (chan : stptr) (s: stack) (h : heap) (trs : traces) (tr : trace) (rexpr : dexpr) n
+       (HProtocol : (forall T, MapsTo p T PM -> ST_trace_strong P (T s) tr))
+       (HFresh    : ~ In chan trs)
+       (HLookup   : method_lookup P C m (Build_Method (a::nil) c rexpr))
+       (HSem      : sc P PM n (stack_add a (vst chan) (stack_empty _)) heap_unit (add chan tr (empty _)) None),
+       start_sem C m x p c sc P PM (S n) s h trs None
+  | start_failE   : forall (P : Prog_wf) PM (a : var) (chan : stptr) (s rs: stack) (h rh : heap) (trs rtrs : traces) (tr : trace) (rexpr : dexpr) n
+      (HProtocol : (forall T, MapsTo p T PM -> ST_trace_strong P (T s) tr)) 
+       (HFresh    : ~ In chan trs)
+       (HLookup   : method_lookup P C m (Build_Method (a::nil) c rexpr))
+       (HSem      : sc P PM n (stack_add a (vst chan) (stack_empty _)) heap_unit (add chan tr (empty _)) (Some (rs, (rh, rtrs))))
+       (HOngoing  : ~ MapsTo chan tinit rtrs),
+       start_sem C m x p c sc P PM (S n) s h trs None
+  | start_ok      : forall (P : Prog_wf) PM (a : var) (chan : stptr) (s rs: stack) (h rh : heap) (trs : traces) (tr : trace) (rexpr : dexpr) n
+       (HProtocol : (forall T, MapsTo p T PM -> ST_trace_strong P (T s) tr)) 
+       (HFresh    : ~ In chan trs)
+       (HLookup   : method_lookup P C m (Build_Method (a::nil) c rexpr))
+       (HSem      : sc P PM n (stack_add a (vst chan) (stack_empty _)) heap_unit (add chan tr (empty _)) (Some (rs, (rh, (add chan tinit (empty _)))))),
+       start_sem C m x p c sc P PM (S n) s h trs (Some ((stack_add x (vst chan) s), (h, (add chan (dual tr) trs)))).
+  Program Definition start_cmd C m x p c sc := Build_semCmd (start_sem C m x p c sc) _ _.
   Next Obligation.
     intros H; inversion H.
   Qed.
@@ -470,9 +484,9 @@ Require Import Compare_dec.
       semantics (csend x y) (send_cmd x y)
   | semrecv : forall v x,
       semantics (crecv v x) (recv_cmd v x)
-  | semstart : forall (x : var) (C : class) m c sc
+  | semstart : forall (x : var) (C : class) m (p : protocol) c sc
       (HSem  : semantics c sc),
-      semantics (cstart x C m) (start_cmd C m x c sc)
+      semantics (cstart x C m p) (start_cmd C m x p c sc)
   .
 
   Definition c_not_modifies c x :=
@@ -482,53 +496,53 @@ Require Import Compare_dec.
      ~ SS.In x (modifies c) -> c_not_modifies c x.
   Proof.
     induction c; simpl in *; intros HNM; intros sc HSem; inversion_clear HSem.
-    + rewrite SS'.singleton_iff in HNM; intros P s s0 h h0 t t0 n HAsgn;
+    + rewrite SS'.singleton_iff in HNM; intros P PM s s0 h h0 t t0 n HAsgn;
       simpl in *; inversion HAsgn; subst.
       rewrite stack_lookup_add2; trivial.
-    + intros P s s0 h h0 t t0 n HSkip; simpl in *; inversion HSkip; subst; trivial.
-    + intros P s s0 h h0 t t0 n HSeq; simpl in *; inversion HSeq; subst.
+    + intros P PM s s0 h h0 t t0 n HSkip; simpl in *; inversion HSkip; subst; trivial.
+    + intros P PM s s0 h h0 t t0 n HSeq; simpl in *; inversion HSeq; subst.
       transitivity (s2 x).
       * eapply IHc1; [| eassumption | eassumption]; intros HIn; apply HNM;
         rewrite SS'.union_iff; auto.
       * eapply IHc2; [| eassumption | eassumption]; intros HIn; apply HNM;
         rewrite SS'.union_iff; auto.
-    + intros P s s0 h h0 t t0 n HND; simpl in *; inversion HND; subst; clear HND.
-      * inversion H5; subst.
-        apply assume_inv in H7; destruct H7; subst.
+    + intros P PM s s0 h h0 t t0 n HND; simpl in *; inversion HND; subst; clear HND.
+      * inversion H6; subst.
+        apply assume_inv in H8; destruct H8; subst.
         eapply IHc1; [| eassumption | eassumption]; intros HIn; apply HNM;
           rewrite SS'.union_iff; auto.
-      * inversion H5; subst.
-        apply assume_inv in H7; destruct H7; subst.
+      * inversion H6; subst.
+        apply assume_inv in H8; destruct H8; subst.
         eapply IHc2; [| eassumption | eassumption]; intros HIn; apply HNM;
         rewrite SS'.union_iff; auto.
-    + intros P s s0 h h0 t t0 n HKl; simpl in *; inversion HKl; subst; clear HKl.
-      apply assume_inv in H8; destruct H8; destruct H0; subst; simpl in *.
-      remember (Some (s0, (h0, t0))); induction H6; subst;
+    + intros P PM s s0 h h0 t t0 n HKl; simpl in *; inversion HKl; subst; clear HKl.
+      apply assume_inv in H9; destruct H9; destruct H0; subst; simpl in *.
+      remember (Some (s0, (h0, t0))); induction H7; subst;
         [inversion Heqo; trivial | discriminate | discriminate |].
       transitivity (s1 x); simpl in *.
       * inversion H; subst; clear H.
-        apply assume_inv in H8; destruct H8; subst.
+        apply assume_inv in H9; destruct H9; subst.
         eapply IHc; eassumption.
       * apply IHkleene_sem; assumption.
-    + intros P s s0 h h0 t t0 n HWr; simpl in *; inversion HWr; subst; reflexivity.
-    + rewrite SS'.singleton_iff in HNM; intros P s s0 h h0 t t0 n HRd; simpl in *;
+    + intros P PM s s0 h h0 t t0 n HWr; simpl in *; inversion HWr; subst; reflexivity.
+    + rewrite SS'.singleton_iff in HNM; intros P PM s s0 h h0 t t0 n HRd; simpl in *;
       inversion HRd; subst; rewrite stack_lookup_add2; trivial.
-    + rewrite SS'.singleton_iff in HNM; intros P s s0 h h0 t t0 n Hrd; simpl in *.
+    + rewrite SS'.singleton_iff in HNM; intros P PM s s0 h h0 t t0 n Hrd; simpl in *.
       inversion Hrd; subst. rewrite stack_lookup_add2; [reflexivity | assumption].
-    + intros P s s0 h h0 t t0 n Hrd; simpl in *; inversion Hrd; reflexivity.
-    + rewrite SS'.singleton_iff in HNM; intros P s s0 h h0 t t0 n Hrd; simpl in *.
+    + intros P PM s s0 h h0 t t0 n Hrd; simpl in *; inversion Hrd; reflexivity.
+    + rewrite SS'.singleton_iff in HNM; intros P PM s s0 h h0 t t0 n Hrd; simpl in *.
       inversion Hrd; subst. rewrite stack_lookup_add2; [reflexivity | assumption].
-    + rewrite SS'.singleton_iff in HNM; intros P s s0 h h0 t t0 n HCl; simpl in *;
+    + rewrite SS'.singleton_iff in HNM; intros P PM s s0 h h0 t t0 n HCl; simpl in *;
       inversion HCl; subst; rewrite stack_lookup_add2; trivial.
-    + rewrite SS'.singleton_iff in HNM; intros P s s0 h h0 t t0 n HCl; simpl in *;
+    + rewrite SS'.singleton_iff in HNM; intros P PM s s0 h h0 t t0 n HCl; simpl in *;
       inversion HCl; subst; rewrite stack_lookup_add2; trivial.
-    + rewrite SS'.singleton_iff in HNM; intros P s s0 h h0 t t0 n HCl; simpl in *;
+    + rewrite SS'.singleton_iff in HNM; intros P PM s s0 h h0 t t0 n HCl; simpl in *;
       inversion HCl; subst; rewrite stack_lookup_add2; trivial.
-    + intros P s s0 h h0 t t0 n HAs; inversion HAs; subst; reflexivity.
-    + intros P s s0 h h0 t t0 n HAs; inversion HAs; subst; reflexivity.
-    + rewrite SS'.singleton_iff in HNM; intros P s s0 h h0 t t0 n HCl; simpl in *;
+    + intros P PM s s0 h h0 t t0 n HAs; inversion HAs; subst; reflexivity.
+    + intros P PM s s0 h h0 t t0 n HAs; inversion HAs; subst; reflexivity.
+    + rewrite SS'.singleton_iff in HNM; intros P PM s s0 h h0 t t0 n HCl; simpl in *;
       inversion HCl; subst; rewrite stack_lookup_add2; trivial.
-    + rewrite SS'.singleton_iff in HNM; intros P s s0 h h0 t t0 n HCl; simpl in *;
+    + rewrite SS'.singleton_iff in HNM; intros P PM s s0 h h0 t t0 n HCl; simpl in *;
       inversion HCl; subst; rewrite stack_lookup_add2; trivial.
   Qed.
 
@@ -554,7 +568,7 @@ End Commands.
   Local Transparent ILPre_Ops.
   Local Transparent ILFun_Ops.
 
-  Definition triple (P Q : sasn) (c : cmd) :=
+  Definition triple (P Q : psasn) (c : cmd) :=
     Forall sc : semCmd, (semantics c sc) ->> {{P}} sc {{Q}}.
 
   Notation " '{[' P ']}' c '{[' Q ']}' " := (triple P Q c) (at level 89,
@@ -571,14 +585,14 @@ End Commands.
 
 Open Scope open_scope.
 
-  Definition method_spec C m (ps : list var) (rn : var) (P Q : sasn) := (
+  Definition method_spec C m (ps : list var) (rn : var) (P Q : psasn) := (
     NoDup (rn :: ps) /\\
     Exists ps' : (list var), Exists c : cmd, Exists re : dexpr,
       [prog] (fun X : Prog_wf => method_lookup X C m (Build_Method ps' c re)
         /\ length ps = length ps' /\
         (forall x, List.In x ps' -> ~ SS.In x (modifies c)))
-      //\\ {[ P //! zip ps (List.map var_expr ps') ]}
-         c {[ Q //! zip (rn :: ps) (eval re :: (List.map var_expr ps'))]}
+      //\\ {[ psasn_subst P (substl_trunc_aux (zip ps (List.map var_expr ps'))) ]}
+         c {[ psasn_subst Q (substl_trunc_aux (zip (rn :: ps) (eval re :: (List.map var_expr ps'))))]}
     ).
 
   Notation " C ':.:' m |-> ps {{ P }}-{{ r , Q }} " :=
@@ -608,10 +622,10 @@ Open Scope open_scope.
   Qed.
 
 
-  Lemma c_triple_zero P (p q : sasn) (c : cmd) :
+  Lemma c_triple_zero P (p q : psasn) (c : cmd) :
     ({[ p ]} c {[ q ]}) P 0.
   Proof.
-    intros sc n Hn Q HPQ sem R k m s h t HQR Hk Hv Hp.
+    intros sc n Hn Q HPQ sem R PM k m s h t HQR Hk Hv Hp.
     assert (m = 0) by omega.
     assert (k = 0) by omega.
     subst. split.
@@ -639,13 +653,13 @@ Open Scope open_scope.
 
 Section StructuralRules.
 
-  Lemma triple_false (G : spec) (Q : sasn) c :
+  Lemma triple_false (G : spec) (Q : psasn) c :
     G |-- {[lfalse]} c {[Q]}.
   Proof.
     intros n; simpl in *; intros; destruct H4.
   Qed.
 
-  Lemma roc (P P' Q Q' : sasn) c (G : spec)
+  Lemma roc (P P' Q Q' : psasn) c (G : spec)
     (HPre  : P  |-- P')
     (HPost : Q' |-- Q)
     (Hc    : G  |-- {[P']} c {[Q']}) :
@@ -656,7 +670,7 @@ Section StructuralRules.
     lforallL sc. apply lpropimplL; [assumption|]. apply rule_of_consequence; assumption.
   Qed.
 
-  Lemma roc_pre (P P' Q : sasn) c G
+  Lemma roc_pre (P P' Q : psasn) c G
     (HPre : P |-- P')
     (Hc   : G |-- {[P']} c {[Q]}) :
     G |-- {[P]} c {[Q]}.
@@ -664,7 +678,7 @@ Section StructuralRules.
   	eapply roc; eassumption || reflexivity.
   Qed.
 
-  Lemma roc_post (P Q Q' : sasn) c G
+  Lemma roc_post (P Q Q' : psasn) c G
     (Hc : G  |-- {[P]} c {[Q']})
     (HPost : Q' |-- Q) :
     G |-- {[P]} c {[Q]}.
@@ -672,10 +686,10 @@ Section StructuralRules.
     eapply roc; eassumption || reflexivity.
   Qed.
   
-  Lemma rule_frame_ax_list P Q R c (xs: list var)
+  Lemma rule_frame_ax_list (P Q : psasn) (R : sasn) c (xs: list var)
     (HMod : forall x, ~ List.In x xs -> c_not_modifies c x) :
     {[ P ]} c {[ Q ]} |--
-    {[ P ** R ]} c {[ Q ** Exists vs, apply_subst R (subst_fresh vs xs) ]}.
+    {[ P ** embed R ]} c {[ Q ** Exists vs, embed (apply_subst R (subst_fresh vs xs)) ]}.
   Proof.
     unfold triple. lforallR sc; apply lpropimplR; intro Hsc. lforallL sc. 
     apply lpropimplL; [assumption|].
@@ -685,23 +699,23 @@ Section StructuralRules.
   Definition subst_mod_asn (R: sasn) (c: cmd) : sasn :=
     Exists vs, apply_subst R (subst_fresh vs (SS.elements (modifies c))).
 
-  Lemma rule_frame_ax P Q R c : 
+  Lemma rule_frame_ax (P Q : psasn) (R : sasn) c : 
     {[ P ]} c {[ Q ]} |--
-    {[ P ** R ]} c {[ Q ** subst_mod_asn R c ]}.
+    {[ P ** embed R ]} c {[ Q ** embed (subst_mod_asn R c) ]}.
   Proof.
     apply rule_frame_ax_list. intros x HnotIn. apply modifies_syn_sem.
     rewrite SS'.In_elements_iff. assumption.
   Qed.
 
-  Lemma rule_frame P Q R c G 
+  Lemma rule_frame (P Q : psasn) (R : sasn) c G 
     (HPre : G |-- {[P]} c {[Q]}) :
-    G |-- {[ P ** R ]} c {[ Q ** subst_mod_asn R c ]}.
+    G |-- {[ P ** embed R ]} c {[ Q ** embed (subst_mod_asn R c) ]}.
   Proof.
     intros; rewrite <- rule_frame_ax; assumption.
   Qed.
   Implicit Arguments rule_frame [[P] [Q] [R] [c] [G]].
 
-  Lemma exists_into_precond2 {A} (P: A -> sasn) c q :
+  Lemma exists_into_precond2 {A} (P: A -> psasn) c q :
     (Forall x, {[P x]} c {[q]}) -|- {[Exists x, P x]} c {[q]}.
   Proof.
     unfold triple; setoid_rewrite <- exists_into_precond; split.
@@ -711,6 +725,7 @@ Section StructuralRules.
       lforallL sc. apply lpropimplL; [assumption | lforallL x; reflexivity].
   Qed.
   
+  (* fangel, psasn 
   Lemma existentialise_triple (x : var) (P Q : sasn) c (G : spec) 
 	(H : forall (v : val), G |-- {[@lembedand vlogic sasn _ _ (open_eq (x/V) (`v)) P]} c {[Q]}) :
     G |-- {[P]} c {[Q]}.
@@ -718,5 +733,6 @@ Section StructuralRules.
     eapply roc_pre; [apply existentialise_var with (x0 := x)|].
     rewrite <- exists_into_precond2. lforallR y. apply H.
   Qed.
+  *)
 
 End StructuralRules.
