Java/src/Logic/ProtocolLogic.v
@@ -1,0 +1,88 @@
+Require Import Rel Open ILogic ILInsts BILogic BILInsts IBILogic SepAlg SepAlgMap
+               UUSepAlg SepAlgInsts OpenILogic Pure ILEmbed PureInsts Subst Stack.
+Require Import Maps MapInterface MapFacts.
+Require Import Lang ST AssertionLogic SpecLogic Util Program.
+
+Definition PM := Map [protocol, @open var _ ST].
+
+Definition psasn := PM -> sasn.
+
+Local Transparent ILPre_Ops.
+Local Transparent ILFun_Ops.
+Local Transparent BILPre_Ops.
+Local Transparent BILFun_Ops.
+
+Program Definition psasn_subst (P : psasn) (sub : subst) : psasn := 
+  fun PM s => mk_tasn (fun trs => mk_asn (fun Pr k h => P PM (stack_subst s sub) trs Pr k h) _ _ _) _.
+Next Obligation.
+  solve_model H.
+  congruence.
+Defined.
+Next Obligation.
+  solve_model H0.
+  congruence.
+Defined.
+Next Obligation.
+  solve_model H0.
+  congruence.
+Defined.
+Next Obligation.
+  solve_model H0.
+  congruence.
+Defined.
+
+Program Definition ST_exists (p : protocol) (T : open ST) : psasn :=
+  fun PM s => mk_tasn (fun trs => mk_asn (fun P k h =>
+    MapsTo p T PM
+  ) _ _ _) _.
+
+Local Existing Instance ILPre_Ops.
+Local Existing Instance ILPre_ILogic.
+Local Existing Instance EmbedOpId.
+Local Existing Instance EmbedId.
+Local Existing Instance ILFun_Ops.
+Local Existing Instance ILFun_ILogic.
+Local Existing Instance SAIBIOps.
+Local Existing Instance SAIBILogic.
+Local Existing Instance BILPre_Ops.
+Local Existing Instance IBILPreLogic.
+Local Existing Instance BILFun_Ops.
+Local Existing Instance IBILFunLogic.
+
+Local Existing Instance MapSepAlgOps.
+Local Existing Instance MapSepAlg.
+Local Existing Instance MapEquiv.
+Local Existing Instance EquivPreorder.
+Local Existing Instance UUMapSepAlg.
+Local Existing Instance SepAlgOps_prod.
+Local Existing Instance SepAlg_prod.
+Local Existing Instance UUSepAlg_prod.
+
+Instance ILogicOpsPSasn    : ILogicOps psasn    := _.
+Instance ILogicPSasn       : ILogic psasn       := _.
+Instance BILOperatorsPSasn : BILOperators psasn := _.
+Instance BILogicPSasn      : BILogic psasn      := _.
+Instance IBILogicPSasn     : IBILogic psasn     := _.
+
+Local Existing Instance EmbedILFunDropOp.
+Local Existing Instance EmbedILFunDrop.
+Local Existing Instance EmbedILFunOp.
+Local Existing Instance EmbedILFun.
+Local Existing Instance EmbedILPreOp.
+Local Existing Instance EmbedILPre.
+
+Local Existing Instance SABIOps.
+Local Existing Instance SABILogic.
+Local Existing Instance pureop_bi_sepalg.
+
+Instance EmbedPSasnPropOp : EmbedOp Prop psasn := _.
+Instance EmbedPSasnProp   : Embed Prop psasn   := _.
+
+Instance EmbedPSasnPureOp : EmbedOp vlogic psasn := _.
+Instance EmbedPSasnPure   : Embed vlogic psasn   := _.
+
+Instance EmbedPSasnSpecOp : EmbedOp spec psasn := _.
+Instance EmbedPSasnSpec   : Embed spec psasn   := _.
+
+Instance EmbedPSasnSasnOp : EmbedOp sasn psasn := _. 
+Instance EmbedPSasnSasn   : Embed sasn psasn := _.
