Java/src/Semantics/SemCmdRules.v
@@ -1,5 +1,5 @@
 Require Import SemCmd ILogic BILogic ILInsts BILInsts. 
-Require Import OpenILogic Later AssertionLogic SpecLogic ILEmbed Open.
+Require Import OpenILogic Later ProtocolLogic AssertionLogic SpecLogic ILEmbed Open.
 Require Import Stack Subst Lang Util List.
 Require Import FunctionalExtensionality Traces.
 
@@ -15,53 +15,54 @@ Open Scope open_scope.
     Local Transparent BILFun_Ops.
     Local Transparent ILLaterPreOps.
     Local Transparent ILLaterNatOps.
-
+    Local Transparent EmbedPSasnSasnOp.
+    Local Transparent EmbedILFunDropOp.
 
 Section Rules.
 
   Section StructuralRules.
 
-    Lemma rule_of_consequence (P P' Q Q' : sasn) (c : semCmd)
+    Lemma rule_of_consequence (P P' Q Q' : psasn) (c : semCmd)
       (HPre  : P  |-- P')
       (HPost : Q' |-- Q ) :
       {{P'}}c{{Q'}} |-- {{P}}c{{Q}}.
     Proof.
-      intros n Pr Hc Pr' m k s h t HPr Hmn Hkm HP; simpl.
-      destruct (Hc _ _ _ s h t HPr Hmn Hkm) as [HSafe HQ].
+      intros n Pr Hc Pr' PM m k s h t HPr Hmn Hkm HP; simpl.
+      destruct (Hc _ PM _ _ s h t HPr Hmn Hkm) as [HSafe HQ].
       + apply HPre; apply HP.
-      + split; [apply HSafe|intros t' h' s' H]. (* split. *)
-        - apply HPost. specialize (HQ _ _ _ H). apply HQ.
-        (* - specialize (HQ _ _ _ H). apply HQ. *)
+      + split; [apply HSafe|intros t' h' s' H].
+        apply HPost. specialize (HQ _ _ _ H). apply HQ.
     Qed.
 
     Definition not_modifies (c : semCmd) (x : var) : Prop :=
-      forall PP s s' h h' t t' n (HSem : c PP n s h t (Some (s', (h', t')))),
+      forall PP PM s s' h h' t t' n (HSem : c PP PM n s h t (Some (s', (h', t')))),
         s x = s' x.
-
-    Lemma frame_rule : forall P Q R c (xs: list var)
+        
+    Lemma frame_rule : forall (P Q : psasn) (R : sasn) c (xs: list var)
       (HMod : forall x, ~ In x xs -> not_modifies c x),
       {{ P }} c {{ Q }} |--
-      {{ P ** R }} c {{ Q ** Exists vs, apply_subst R (subst_fresh vs xs) }}.
+      {{ P ** embed R }} c {{ Q ** Exists vs, embed (apply_subst R (subst_fresh vs xs)) }}.
     Proof.
       intros.
-      intros PP n HSpec PP' ? ? ? ? ? HPP' Hmn Hkm [h1 [h2 [HSub [HP HR]]]]; split.
+      intros PP n HSpec PP' ? ? ? ? ? ? HPP' Hmn Hkm [h1 [h2 [HSub [HP HR]]]]; split.
       (* safety *)
-      { destruct (HSpec _ m k s h t HPP' Hmn Hkm) as [HS _]; [ | assumption].
+      { destruct (HSpec _ PM m k s h t HPP' Hmn Hkm) as [HS _]; [ | assumption].
         solve_model HP. exists h2; apply HSub.
       }
       (* correctness *)
       intros ? ? ? HSem. 
-      destruct (@cmd_frame c PP' s s' h h' h2 h1 k t t') as [h'' [HBig Hc]]. 
+      destruct (@cmd_frame c PP' PM s s' h h' h2 h1 k t t') as [h'' [HBig Hc]]. 
       + assumption.
       + intros l Hle.
-        destruct (HSpec _ m l s h1 t HPP' Hmn) as [HS _]; [ omega | assumption |].
+        destruct (HSpec _ PM m l s h1 t HPP' Hmn) as [HS _]; [ omega | assumption |].
         apply HS.
       + assumption.
-      + destruct (HSpec _ m k s h1 t HPP' Hmn Hkm) as [_ HC]. 
+      + destruct (HSpec _ PM m k s h1 t HPP' Hmn Hkm) as [_ HC]. 
         * apply HP.
         * specialize (HC t' h'' s' Hc).
           exists h'', h2, HBig. split; [assumption |].
-          simpl. exists s. unfold apply_subst.
+          simpl. exists s. unfold apply_subst, id.
+          simpl in HR; unfold id in HR.
           solve_model HR.
           - unfold Rel.rel, MapInterface.Equal.
             intros x.
@@ -70,7 +71,7 @@ Section Rules.
             unfold stack_subst, subst_fresh.
             destruct (in_dec Rel.dec_eq x xs) as [|HNotIn]; [reflexivity|].
             unfold not_modifies in HMod. 
-            specialize (HMod _ HNotIn _ _ _ _ _ _ _ _ HSem).
+            specialize (HMod _ HNotIn _ PM _ _ _ _ _ _ _ HSem).
             apply HMod.
     Qed.
 
@@ -80,7 +81,7 @@ Section Rules.
       G |-- {{P1 //\\ P2}} c {{Q1 //\\ Q2}}.
     Proof.
       intros n P HPP HG.
-      simpl. intros m k s h t HPP' Hm Hk [HP1 HP2]. split.
+      simpl. intros PM m k s h t HPP' Hm Hk [HP1 HP2]. split.
       + eapply H1; eauto.
       + intros t' h' s' Hsem.
         split; [eapply H1|eapply H2]; eauto.
@@ -92,7 +93,7 @@ Section Rules.
 
     Lemma skip_rule P : |-- {{P}}skip_cmd {{P}}.
     Proof.
-      intros n Pr HPP Pr' m k s h t _ Hmn Hkm HP; split.
+      intros PM n Pr HPP Pr' m k s h t _ Hmn Hkm HP; split.
       + intros H; inversion H.
       + intros t' h' s' HSem; inversion HSem; subst.
         solve_model HP.
@@ -101,62 +102,60 @@ Section Rules.
     Lemma seq_rule c1 c2 P Q R :
       ({{P}}c1{{Q}} //\\ {{Q}}c2{{R}}) |-- {{P}}seq_cmd c1 c2{{R}}.
     Proof.
-      intros Pr n [Hc1 Hc2] Pr' k m s h t HPP' Hmn Hkm HP; split.
+      intros Pr n [Hc1 Hc2] Pr' PM k m s h t HPP' Hmn Hkm HP; split.
       + intros HFail; inversion HFail; subst; clear HFail.	
-        * destruct (Hc1 _ _ n0 s h t HPP' Hmn) as [HS _];
+        * destruct (Hc1 _ PM _ n0 s h t HPP' Hmn) as [HS _];
           [omega | assumption | apply HS; assumption ].
-        * destruct (Hc1 _ _ n0 s h t HPP' Hmn) as [_ HC]; [omega | assumption |].
+        * destruct (Hc1 _ PM _ n0 s h t HPP' Hmn) as [_ HC]; [omega | assumption |].
           specialize (HC _ _ _ H).
-          destruct (Hc2 _ (k - n0) n' s' h' t' HPP') as [HS _]; [omega | omega | |].
+          destruct (Hc2 _ PM (k - n0) n' s' h' t' HPP') as [HS _]; [omega | omega | |].
           apply HC. 
           apply HS; exact H0.
       + intros t' h' s' HSem; inversion HSem; subst; clear HSem.
-        destruct (Hc1 _ _  n0 s h t HPP' Hmn) as [_ HC1]; [omega | assumption |].
-        specialize (HC1 _ _ _ H6) (*; destruct HC1 as [HC1 Hst1] *).
-        destruct (Hc2 _ (k - n0) n1 s1 h1 t1 HPP') as [_ HC2]; [omega | omega | |].
+        destruct (Hc1 _ PM _ n0 s h t HPP' Hmn) as [_ HC1]; [omega | assumption |].
+        specialize (HC1 _ _ _ H7).
+        destruct (Hc2 _ PM (k - n0) n1 s1 h1 t1 HPP') as [_ HC2]; [omega | omega | |].
         apply HC1.
-        specialize (HC2 _ _ _ H8) (*; destruct HC2 as [HC2 Hst2] *).
+        specialize (HC2 _ _ _ H9).
         solve_model HC2. 
     Qed.
 
     Lemma nondet_rule c1 c2 P Q:
       ({{P}}c1{{Q}} //\\ {{P}}c2{{Q}}) |-- {{P}}nondet_cmd c1 c2{{Q}}.
     Proof.
-      intros n Pr [Hc1 Hc2] Pr' k m s h t HPP' Hmn Hkm HP; split.
+      intros n Pr [Hc1 Hc2] Pr' PM k m s h t HPP' Hmn Hkm HP; split.
       + intros HFail; inversion HFail; subst; clear HFail.
-        * destruct (Hc1 _ _ n0 s h t HPP' Hmn) as [HS _];
+        * destruct (Hc1 _ PM _ n0 s h t HPP' Hmn) as [HS _];
           [omega | assumption | apply HS; assumption].
-        * destruct (Hc2 _ _ n0 s h t HPP' Hmn) as [HS _];
+        * destruct (Hc2 _ PM _ n0 s h t HPP' Hmn) as [HS _];
           [omega | assumption | apply HS; assumption].
       + intros h1 s1 t1 HSem; inversion HSem; subst; clear HSem.
-        * destruct (Hc1 _ _ n0 s h t HPP' Hmn) as [_ HC]; [omega | assumption |].
-          specialize (HC _ _ _ H5) (*; destruct HC as [HC Hst] *). 
+        * destruct (Hc1 _ PM _ n0 s h t HPP' Hmn) as [_ HC]; [omega | assumption |].
+          specialize (HC _ _ _ H6). 
           solve_model HC.
-          (* split; [ solve_model HC | assumption ]. *)
-        * destruct (Hc2 _ _ n0 s h t HPP' Hmn) as [_ HC]; [omega | assumption |].
-          specialize (HC _ _ _ H5) (*; destruct HC as [HC Hst] *).
+        * destruct (Hc2 _ PM _ n0 s h t HPP' Hmn) as [_ HC]; [omega | assumption |].
+          specialize (HC _ _ _ H6).
           solve_model HC.
     Qed.
 
     Lemma kleene_rule c P:
       {{P}}c{{P}} |-- {{P}} kleene_cmd c {{P}}.
     Proof.
-      intros Pr n Hc Pr' m k s h t HPP' Hmn Hkm Hp; split.
+      intros Pr n Hc Pr' PM m k s h t HPP' Hmn Hkm Hp; split.
       + intros HFail. generalize dependent m. remember None as cfg.
         induction HFail; intros; inversion Heqcfg; subst.
-        * destruct (Hc _ m n0 s h t HPP' Hmn) as [HS _];
+        * destruct (Hc _ PM m n0 s h t HPP' Hmn) as [HS _];
           [omega | assumption | apply HS; assumption].
-        * destruct (Hc _ m n0 s h t HPP' Hmn) as [_ HC]; [omega | assumption |].
+        * destruct (Hc _ PM m n0 s h t HPP' Hmn) as [_ HC]; [omega | assumption |].
           apply IHHFail with (m-n0); [assumption | reflexivity | omega | omega | ].
-          specialize (HC _ _ _ H) (*; destruct HC as [HC Hst] *).
+          specialize (HC _ _ _ H).
           solve_model HC.
       + intros. remember (Some (s', (h', t'))) as cfg. generalize dependent m. 
         induction H; inversion Heqcfg; subst; intros.
         * solve_model Hp.
-          (* split; [ solve_model Hp | intuition ]. *)
-        * destruct (Hc _ m n0 s h t HPP' Hmn) as [_ HC]; [omega | assumption |].
-          specialize (HC _ _ _ H) (*; destruct HC as [HC Hst] *).
-          assert ((((P s') t' P0) ((m - n0) - n1)) h') as H2. 
+        * destruct (Hc _ PM m n0 s h t HPP' Hmn) as [_ HC]; [omega | assumption |].
+          specialize (HC _ _ _ H).
+          assert ((((P PM s') t' Pr0) ((m - n0) - n1)) h') as H2. 
             apply IHkleene_sem; try assumption; try omega. 
           solve_model H2.
     Qed.
@@ -164,17 +163,17 @@ Section Rules.
     Lemma assume_rule P (t : vlogic) :
       |-- {{P}} assume_cmd t {{t /\\ P}}.
     Proof.
-      intros n Pr Hc Pr' m k s h tr HPP' Hmn Hkm Hp; split.
+      intros n Pr Hc Pr' PM m k s h tr HPP' Hmn Hkm Hp; split.
       + intros HFail. inversion HFail.
       + intros tr' h' s' H. remember (Some (s', (h', tr'))) as cfg; induction H.
         inversion Heqcfg; subst; intros.
         split; [assumption|]. solve_model Hp.
     Qed.
 
-    Lemma assert_rule (P : sasn) (p : vlogic) (HPe : P |-- embed p) :
+    Lemma assert_rule (P : psasn) (p : vlogic) (HPe : P |-- embed p) :
       |-- {{P}} assert_cmd p {{P}}.
     Proof.
-      intros n Pr Hc Pr' m k s h t HPP' Hmn Hkm Hp; specialize (HPe _ _ _ _ _ Hp); split.
+      intros n Pr Hc Pr' PM m k s h t HPP' Hmn Hkm Hp; specialize (HPe _ _ _ _ _ _ Hp); split.
       + intros HF; inversion HF; subst; auto.
       + intros t' h' s' HSem; inversion HSem; subst.
         solve_model Hp.
@@ -182,25 +181,25 @@ Section Rules.
 
   End PrimitivesRules.
 
-  Lemma exists_into_precond {A} (P: A -> sasn) c q :
+  Lemma exists_into_precond {A} (P: A -> psasn) c q :
     (Forall x, {{P x}} c {{q}}) -|- {{Exists x, P x}} c {{q}}.
   Proof.
   	split.
-  	+ intros n Pr Hp Pr' m k s h t HPP' Hmn Hkm [x Hxp]; specialize (Hp x); auto.
-  	+ intros n Pr Hp x Pr' m k s h t HPP' Hmn Hkm Hxp.
+  	+ intros n Pr Hp Pr' PM m k s h t HPP' Hmn Hkm [x Hxp]; specialize (Hp x); auto.
+  	+ intros n Pr Hp x Pr' PM m k s h t HPP' Hmn Hkm Hxp.
   	  apply Hp; try assumption. exists x; apply Hxp.
   Qed.
 
   (* Holds only in one direction unless annotations on assertion logic, which is ugly - well, it's happened. - F.
      This is the important direction, though *)
-  Lemma I_precond (SP : spec) (P Q : sasn) c:
+  Lemma I_precond (SP : spec) (P Q : psasn) c:
     (SP -->> {{ P }} c {{ Q }}) -|- {{ SP /\\  P }} c {{ Q }}.
   Proof.
   	split.
-  	+ intros Pr n Hp Pr' m k s h t HPP' Hmn Hkm [HSP HP].
+  	+ intros Pr n Hp Pr' PM m k s h t HPP' Hmn Hkm [HSP HP].
   	  specialize (Hp Pr' HPP' m Hmn HSP).
   	  apply Hp; reflexivity || assumption.
-  	+ intros Pr n Hp Pr' HPP' m Hnm HSP Pr'' k l s h t HPP'' Hkm Hkl HP.
+  	+ intros Pr n Hp Pr' HPP' m Hnm HSP Pr'' PM k l s h t HPP'' Hkm Hkl HP.
   	  apply Hp.
   	  * transitivity Pr'; assumption.
   	  * omega.
